break out the sub1 loop into its own file

arith/sub1.v
@@ -55,34 +55,6 @@ Next Obligation.
   apply (not_even_and_odd (S wildcard')); auto.
 Qed.
 
-Fixpoint sub1_linear_time n :=
-  match n with
-    | 0 => 3
-    | S n' => sub1_time n + sub1_linear_time n' + 7
-  end.
-
-Definition sub1_linear_loop_result (n:nat) (res:nat) (c:nat) :=
-  c = sub1_linear_time n.
-Hint Unfold sub1_linear_loop_result.
-
-Load "sub1_linear_loop_gen.v".
-
-Next Obligation.
-  rename H into SUB1R.
-  destruct SUB1R.
-  omega.
-Qed.
-
-Next Obligation.
-  clear H2 am0 am H3 sub1_linear_loop.
-  rename H1 into SUB1_RESULT.
-  
-  unfold sub1_linear_loop_result in *.
-  destruct SUB1_RESULT.
-  subst an an0 n'.
-  unfold sub1_linear_time; fold sub1_linear_time.
-  replace (S wildcard' - 1) with wildcard'; omega.
-Qed.
 
 Program Fixpoint sub1_time2 (n:nat) {measure n} :=
   match n with
@@ -203,3 +175,4 @@ Proof.
   apply sub1_time3_O_cl_log.
   apply cl_log_O_fl_log.
 Qed.
+
