arith/sub1_linear.v
@@ -1,0 +1,37 @@
+Require Import Braun.monad.monad Braun.common.log.
+Require Import Braun.common.util Braun.common.big_oh Braun.common.le_util.
+Require Import Arith Arith.Even Arith.Div2.
+Require Import Coq.Program.Wf Arith.Even Arith.Div2 Arith Init.Wf.
+Require Import Braun.arith.sub1.
+
+Include WfExtensionality.
+
+Fixpoint sub1_linear_time n :=
+  match n with
+    | 0 => 3
+    | S n' => sub1_time n + sub1_linear_time n' + 7
+  end.
+
+Definition sub1_linear_loop_result (n:nat) (res:nat) (c:nat) :=
+  c = sub1_linear_time n.
+Hint Unfold sub1_linear_loop_result.
+
+Load "sub1_linear_loop_gen.v".
+
+Next Obligation.
+  rename H into SUB1R.
+  destruct SUB1R.
+  omega.
+Qed.
+
+Next Obligation.
+  clear H2 am0 am H3 sub1_linear_loop.
+  rename H1 into SUB1_RESULT.
+  
+  unfold sub1_linear_loop_result in *.
+  destruct SUB1_RESULT.
+  subst an an0 n'.
+  unfold sub1_linear_time; fold sub1_linear_time.
+  replace (S wildcard' - 1) with wildcard'; omega.
+Qed.
+
